update type of flags

examples/pseudo_bool/cp_encoding/cp_to_ilp_primScript.sml
@@ -7,16 +7,13 @@ Libs
 Ancestors
   pbc cp ilp cp_to_ilp
 
-Definition encode_ne_def:
-  encode_ne bnd X Y =
-    [
-      bits_imply bnd [Pos (INR (Ne X Y))] (mk_constraint_ge 1 X (-1) Y 1);
-      bits_imply bnd [Neg (INR (Ne X Y))] (mk_constraint_ge 1 Y (-1) X 1)
-    ]
+Definition ne_var_def[simp]:
+  ne_var name =
+    INR (name, Flag (strlit "ne"))
 End
 
 Definition encode_equal_def:
-  encode_equal bnd Zr X Y =
+  encode_equal bnd Zr X Y name =
   let constr =
     [
       mk_constraint_ge 1 (X) (-1) (Y) 0;
@@ -32,32 +29,33 @@ Definition encode_equal_def:
     MAP (bits_imply bnd [Pos (INL (Ge Z 1))]) constr ++
     [
       bits_imply bnd
-        [Neg (INL (Ge Z 1)); Pos (INR (Ne X Y))]
+        [Neg (INL (Ge Z 1)); Pos (ne_var name)]
           (mk_constraint_ge 1 X (-1) Y 1);
       bits_imply bnd
-        [Neg (INL (Ge Z 1)); Neg (INR (Ne X Y))]
+        [Neg (INL (Ge Z 1)); Neg (ne_var name)]
           (mk_constraint_ge 1 Y (-1) X 1)
     ]
 End
 
 Theorem encode_equal_sem_1:
   valid_assignment bnd wi ∧
+  ALOOKUP cs name = SOME (Prim (Cmpop reif cmp X Y)) ∧
   reify_sem Zr wi
     (varc wi X = varc wi Y) ⇒
-  EVERY (λx. iconstraint_sem x (wi,reify_avar wi))
-    (encode_equal bnd Zr X Y)
+  EVERY (λx. iconstraint_sem x (wi,reify_avar cs wi))
+    (encode_equal bnd Zr X Y name)
 Proof
   rw[reify_sem_def,encode_equal_def]>>
   gvs[AllCasePreds(),reify_avar_def,reify_reif_def,reify_flag_def]
-  >-  intLib.ARITH_TAC
-  >-  intLib.ARITH_TAC
-  >-  intLib.ARITH_TAC
+  >- intLib.ARITH_TAC
+  >- intLib.ARITH_TAC
+  >- intLib.ARITH_TAC
 QED
 
 Theorem encode_equal_sem_2:
   valid_assignment bnd wi ∧
   EVERY (λx. iconstraint_sem x (wi,wb))
-    (encode_equal bnd Zr X Y) ⇒
+    (encode_equal bnd Zr X Y name) ⇒
   reify_sem Zr wi
     (varc wi X = varc wi Y)
 Proof
@@ -65,25 +63,31 @@ Proof
   every_case_tac>>gvs[]
   >-  intLib.ARITH_TAC
   >-  intLib.ARITH_TAC>>
-  Cases_on`wb (INR (Ne X Y))`>>gvs[]
+  rename1`wb (INR f)`>>
+  Cases_on`wb (INR f)`>>gvs[]
   >-  intLib.ARITH_TAC
   >-  intLib.ARITH_TAC
 QED
 
 Definition encode_not_equal_def:
-  encode_not_equal bnd Zr X Y =
-  let constr = encode_ne bnd X Y in
+  encode_not_equal bnd Zr X Y name =
+  let xgty = (mk_constraint_ge 1 X (-1) Y 1) in
+  let ygtx = (mk_constraint_ge 1 Y (-1) X 1) in
   case Zr of
-    NONE => constr
+    NONE =>
+    [
+      bits_imply bnd [Pos (ne_var name)] xgty;
+      bits_imply bnd [Neg (ne_var name)] ygtx
+    ]
   | SOME (INL Z) =>
     encode_ge bnd Z 1 ++
     [
       bits_imply bnd
-        [Pos (INL (Ge Z 1)); Pos (INR (Ne X Y))]
-          (mk_constraint_ge 1 X (-1) Y 1);
+        [Pos (INL (Ge Z 1)); Pos (ne_var name)]
+          xgty;
       bits_imply bnd
-        [Pos (INL (Ge Z 1)); Neg (INR (Ne X Y))]
-          (mk_constraint_ge 1 Y (-1) X 1)
+        [Pos (INL (Ge Z 1)); Neg (ne_var name)]
+          ygtx
     ]
   | SOME (INR Z) =>
     encode_ge bnd Z 1 ++
@@ -94,22 +98,23 @@ Definition encode_not_equal_def:
       ] ++
     [
       bits_imply bnd
-        [Pos (INL (Ge Z 1)); Pos (INR (Ne X Y))]
-          (mk_constraint_ge 1 X (-1) Y 1);
+        [Pos (INL (Ge Z 1)); Pos (ne_var name)]
+          xgty;
       bits_imply bnd
-        [Pos (INL (Ge Z 1)); Neg (INR (Ne X Y))]
-          (mk_constraint_ge 1 Y (-1) X 1)
+        [Pos (INL (Ge Z 1)); Neg (ne_var name)]
+          ygtx
     ]
 End
 
 Theorem encode_not_equal_sem_1:
   valid_assignment bnd wi ∧
+  ALOOKUP cs name = SOME (Prim (Cmpop reif cmp X Y)) ∧
   reify_sem Zr wi
     (varc wi X ≠ varc wi Y) ⇒
-  EVERY (λx. iconstraint_sem x (wi,reify_avar wi))
-    (encode_not_equal bnd Zr X Y)
+  EVERY (λx. iconstraint_sem x (wi,reify_avar cs wi))
+    (encode_not_equal bnd Zr X Y name)
 Proof
-  rw[reify_sem_def,encode_not_equal_def,encode_ne_def]>>
+  rw[reify_sem_def,encode_not_equal_def]>>
   gvs[AllCasePreds(),reify_avar_def,reify_flag_def,reify_reif_def]
   >-  intLib.ARITH_TAC
   >-  intLib.ARITH_TAC
@@ -119,40 +124,42 @@ QED
 Theorem encode_not_equal_sem_2:
   valid_assignment bnd wi ∧
   EVERY (λx. iconstraint_sem x (wi,wb))
-    (encode_not_equal bnd Zr X Y) ⇒
+    (encode_not_equal bnd Zr X Y name) ⇒
   reify_sem Zr wi
     (varc wi X ≠ varc wi Y)
 Proof
-  rw[reify_sem_def,encode_not_equal_def,encode_ne_def]>>
+  rw[reify_sem_def,encode_not_equal_def]>>
   gvs[AllCasePreds(),reify_avar_def,reify_flag_def,reify_reif_def]>>
+  rename1`INR f`>>
   every_case_tac>>gvs[]
   >- (
-    Cases_on`wb (INR (Ne X Y))`>>gvs[]>>
+    Cases_on`wb (INR f)`>>gvs[]>>
     intLib.ARITH_TAC)
   >- (
-    Cases_on`wb (INR (Ne X Y))`>>gvs[]>>
+    Cases_on`wb (INR f)`>>gvs[]>>
     intLib.ARITH_TAC)
   >- (
-    Cases_on`wb (INR (Ne X Y))`>>gvs[]>>
+    Cases_on`wb (INR f)`>>gvs[]>>
     intLib.ARITH_TAC)
 QED
 
 Definition encode_prim_constr_def:
-  encode_prim_constr bnd c =
+  encode_prim_constr bnd c name =
   case c of
     Cmpop Zr cmp X Y =>
       (case cmp of
-        Equal => encode_equal bnd Zr X Y
-      | NotEqual => encode_not_equal bnd Zr X Y
+        Equal => encode_equal bnd Zr X Y name
+      | NotEqual => encode_not_equal bnd Zr X Y name
       | _ => ARB)
   | _ => ARB
 End
 
 Theorem encode_prim_constr_sem_1:
   valid_assignment bnd wi ∧
+  ALOOKUP cs name = SOME (Prim c) ∧
   prim_constr_sem c wi ⇒
-  EVERY (λx. iconstraint_sem x (wi,reify_avar wi))
-    (encode_prim_constr bnd c)
+  EVERY (λx. iconstraint_sem x (wi,reify_avar cs wi))
+    (encode_prim_constr bnd c name)
 Proof
   Cases_on`c`>>
   rw[encode_prim_constr_def,prim_constr_sem_def]
@@ -169,7 +176,7 @@ QED
 
 Theorem encode_prim_constr_sem_2:
   valid_assignment bnd wi ∧
-  EVERY (λx. iconstraint_sem x (wi,wb)) (encode_prim_constr bnd c) ⇒
+  EVERY (λx. iconstraint_sem x (wi,wb)) (encode_prim_constr bnd c name) ⇒
   prim_constr_sem c wi
 Proof
   Cases_on`c`>>
@@ -184,5 +191,4 @@ Proof
     >- metis_tac[encode_not_equal_sem_2]
     >> cheat)
 QED
-
 
